<!--  <./segments/305-left.md> -->
[↗](../images/segments/305-left.png)


```
Γ ⟶ Θ, Λ   Σ ⟶ Π
―――――――――――――――――― mix
Γ, Σ*⟶ Θ*, Λ*, Π  possibly several
                    interchanges and
                    thinnings
                    B, Δ ⟶ Λ   Σ ⟶ Π
                    ――――――――――――――――― mix
                    B, Δ, Σ*⟶ Λ*, Π
――――――――――――――――――――――――――――――――――― possibly several
A ⊃ B, Γ, Σ*, Δ, Σ*⟶ Θ*, Π, Λ*, Π  contractions and
A ⊃ B, Γ, Δ, Σ*⟶ Θ*, Λ*, Π         interchanges.

Both mixes may be eliminated by virtue of the
induction hypothesis.

If the Σ-formula **M** does not occur in both Θ
and Λ simultaneously. It must occur in one of them.
We consider the case of **M** occurring in Λ but not
in Θ; the alternative case is completely analogous.

We transform the end of the derivation into:

                    B, Δ ⟶ Λ   Σ ⟶ Π
Γ ⟶ Θ, Λ           ――――――――――――――――― mix
                    B, Δ, Σ*⟶ Λ*, Π
―――――――――――――――――――――――――――――――――― ⊃-IΛ
A ⊃ B, Γ, Δ, Σ*⟶ Θ, Λ*, Π

The mix may be eliminated by virtue of the
induction hypothesis.

3.2. *Proof of the Hauptsatz for LJ-derivations.*

In order to transform an *LJ*-derivation into an
*LJ*-derivation *without cuts*, we apply *exactly the same
procedure* as for *LK*-derivations.

Since an *LJ*-derivation is a special case of an
*LK*-derivation, it is clear that the transformation
can be carried out. We have only to convince
ourselves that with every transformation step an
*LJ*-derivation becomes another *LJ*-derivation, i.e.,
that the consequents of the transformed derivation
do not contain more than one S-formula in the
succedent, given that this was the case before.

We therefore examine each step of the trans-
formation from that point of view.

3.21. Replacement of cuts by mixes. An *LJ*-cut
runs:

        Γ ⟶ D   D, Δ ⟶Λ
        ―――――――――――――――,
             Γ, Δ ⟶ Λ

where Λ contains at most one S-formula. We
transform this cut into:

Γ ⟶ D      D, Δ ⟶ Λ
――――――――――――――――――― mix
      Γ, Δ*⟶ Λ       possibly several interchanges
      ――――――――― Δ and thinnings in the ante-
      Γ, Δ ⟶Λ       cedent.

This replacement gives us a new *LJ*-derivation.

3.22. By replacing the free choice variable (3.10)
we trivially get another *LJ*-derivation from a
previous one.
```

<!--  <./segments/305-right.md> -->
[↗](../images/segments/305-right.png)


3.23. The transformation proper (3.11 and 3.12).
We have to show for each of the cases 3.111 to
3.122.12 that the given transformations do not
introduce any sequents with more than one Σ-
formula in the succedent.

3.231. Let us begin with the cases 3.11:
In the cases 3.111, 3.113.1, 3.113.31, 3.113.35
and 3.113.36, only such formulae occur in each
succedent of the sequent of a new derivation as
already occurred in the succedent of the sequent of
the original derivation.

Essentially the same applies in 1.113.33. The
only difference is an additional substitution of free
object variables, which does not, of course, alter
the number of succedent formulae of a sequent.

Cases 3.112, 3.113.32, and 3.113.34 were dealt
with symmetrically to cases 3.111, 3.113.1,
3.113.31, and 3.113.33, i.e., in order to get one case
from another, we read the schemata from right to
left instead of from left to right (as well as changing
logical symbols, a process which is here of no
consequence). Hence in the antecedent of one case
we do precisely the same as in the succedent of
another. For the antecedents of cases 3.111, 3.113.1,
3.113.31 and 3.113.33, the same applies as for the
succedents, viz., in every antecedent of a sequent of
the new derivation only such formulae occur as
already occurred in an antecedent of a sequent of
the original derivation.

This disposes of all symmetric cases: 3.112,
3.113.2, 3.113.32 and 3.113.34.

3.23. Now let us look at the cases, 3.12:

3.232.1. For the cases 3.121 it holds generally
that Σ* is empty, since in Π → Σ, Σ must contain
only *one* formula, and this formula must be equal
to **M**.

It is now obvious that in every succedent of a
sequent only such formulae occur as already
occurred in the succedent of a sequent of the
original derivation.

3.232.2. In the cases 3.122 it is somewhat more
difficult to see that from an *LJ*-derivation we
always get another *LJ*-derivation. We must
direct our attention, as we have already done in
considering symmetric cases, to the *antecedents* in
the schemata 3.121.

At this point we distinguish two further sub-
cases:

3.232.21. The case which is symmetric to 3.121.1
is trivial, since in every antecedent of a sequent of
the new derivation (in case 3.121.1) only such
formulae occur as already occurred in an ante-
cedent of a sequent of the original derivation.

